\subsection{Задачи}
	
	Для следующих уравнений построить общее решение:
	\begin{multicols}{2}
		\begin{enumtasks}

			\item \( xy' = y + x^2 \cos{x} \) 														% \frac{y}{x} = \sin{x} + C
			\item \( xy' = y - 2x^2 \cosec{\frac{y}{x}} \) 											% \cos{\frac{y}{x}} = 2x + C
			\item \( 3x^2 y' + 3xy = x - 1 + x\ln{x} \) 											% 3xy + \pares{1 - x} \cdot \ln{x} = C
			\item \( 3xy' + 3y = 2x \cos^2{xy} \) 													% 3 \tan{xy} = x^2 + C
			\item \( xy - x^2y' = xyy' - y^2 \) 													% \frac{x}{y} + \ln{\frac{x}{y}} = C
			\item \( x^4 y' - 2x^3 y = y^2 \) 														% \frac{x^2}{y} = \frac{1}{x} + C
			\item \( 2y^2 y' \cos{y} = xy' - y \) 													% \frac{x}{y} + 2 \sin{y} = C
			\item \( xy^2 y' + x^2 y = x^3y' + 2x^3 y^2 + y^3 \) 									% x^2 + y^2 - x^3 y = Cxy
			\item \( 2x^2 y y' + xy^2 = x - 1 \) 													% xy^2 = x - \ln{x} + C
			\item \( xy' e^{xy} = e^{-x} - ye^{xy} \)												% e^{xy} + e^{-x} = C
			\item \( xy' - 3y + 2x^5 = 0 \) 														% \frac{y}{x^3} + x^2 = C
			\item \( xy' - 3y = 3x^4 y^2 y' - 2x^5 \) 												% x^2 - y^3 + \frac{y}{x^3} = C
			\item \( 3x^5 y + xy^2 y' = x^6 y' + 2y^3 \) 											% x^5 + y^2 = C x^2 y
			\item \( y^3 + xy^2 y' + 3y = 3xy' \) 													% xy + \frac{3x}{y} = C
			\item \( 2x^3 y' + x^4 = 4x^2 y + y^2 \) 												% \frac{y - x^2}{y + x^2} = Cx
			\item \( x^4 y' + 3x^3 y = \ln{x} + 1 \) 												% x^3 y = x \ln{x} + C
			\item \( x^5 y' = 2x^4 y + y^2 \cos^2{\frac{x^2}{y}} \)									% 2 \tan{\frac{x^2}{y}} = \frac{1}{x^2} + C
			\item \( y' \cos{ye^{x}} = 1 - y \cos{ye^{x}} \)										% \sin{ye^{x}} - e^{x} = C
			\item \( y' = 2\sqrt{x + y} \cdot \pares{y' + 1} \cdot \cos{\pares{x + y}} - 1 \)		% \sqrt{x + y} - \sin{\pares{x + y}} = C
			%-----------------
			\item \( \pares{x + y} \cdot y' = x - y \)												% y^2 + 2xy = C + x^2
			\item \( y' = \frac{x + 2y}{2x - y} \)													% \ln\pares{x^2 + y^2} - 4 \arctan{\frac{y}{x}} = C
			\item \( y' = - \frac{y + 2}{x + 6y - 3} \) 											% xy + 2x + 3y^2 - 3y = C
			\item \( xy' + 2x + y + 4 = \pares{y + 1} \cdot y' \) 									% \pares{y - x + 1}^2 = x^2 + 10x + C
			\item \( \pares{x - 3y} \cdot y' = x - y - y' + 4 \) 									% x^2 - 2xy + 4x + 3y^2 - 2y = C
			\item \( \pares{7x + 9y - 3} \cdot y' = 7x + 9y + 1 \) 									% 4y - \ln\pares{28x + 36y - 3} = 4x + C
			\item \( y' = \frac{9x - 5y + 9}{5x - 3y + 1} \) 										% 10xy - 3y^2 + 2y - 9x^2 - 18x = C
			\item \( \pares{1 - 3x} \cdot y' = 9x + 5y - 7 \)										% \pares{45x + 40y - 47}^{3} \cdot \pares{3x - 1}^{5} = C
			\item \( 2x + 4y + 2xy' + 4yy' + 2y' + 1 = 0 \) 										% 2x + 2y + \ln\pares{x + 2y} = C
			\item \( y' =  \frac{3x - y + 1}{x + 9y + 4} \)											% 2xy + 9y^2 + 8y = 3x^2 + 2x + C
			\item \( y' =  \frac{2x - 9y + 30}{9x - 16y + 37} \)									% \pares{8y - x - 29} \cdot \pares{y - x - 1} = C
			\item \( y' =  \frac{9x + 7y + 44}{x - y - 4} \)										% \ln\pares{y + 3x + 8} + \frac{ 4x + 4 }{y + 3x + 8} = C
			\item \( \pares{6x + 10} \cdot y' + \pares{5y + 3} = 2yy' \)							% \pares{33x - 6y + 58}^{5} \cdot \pares{5y + 3}^{6} = C
			\item \( y' = \frac{6x - y + 9}{6x - y - 9} \)											% \pares{30x - 5y - 63}^{18} = C \cdot e^{5\pares{y - x}}
			\item \( 4y' \cdot \pares{2x + y + 3} = 4y - x - 33 \)									% \ln\pares{2y + x - 9} = \frac{3x + 15}{2y + x - 9} + C
			\item \( \pares{x + 14} \cdot y' + 42 = 5x - y \cdot \pares{1 - 3y'} \)					% \pares{y - x + 14} \cdot \pares{3y + 5x - 14} = C

		\end{enumtasks}
	\end{multicols}
