\subsection{Задачи}
	
	Для следующих уравнений построить общее решение:
	\begin{multicols}{2}
		\begin{enumtasks}

			\label{firstorder:to_linear}
			\item \( y' e^{y} + x = e^{y} + 1 \)																		% e^{y} = Ce^{x} + x
			\item \( 2xy' + y = y^3\sin{x} - xy^3 \cos{x} \)															% \frac{1}{y^2} = Cx + \sin{x}
			\item \( 3xy^2 y' - x^2 \cos{x} = y^3 \)																	% y^3 = Cx + x \sin{x}
			\item \( y' e^{y} + e^{-y} = \frac{e^{y}}{x} \)																% e^{2y} = Cx^2 + 2x
			\item \( xy' = y - y^2 \pares{x + 1} e^{x} \)																% \frac{x}{y} - xe^{x} = C
			\item \( xy' + y = 4 \sqrt{xy} \)																			% \sqrt{xy} = C + 2x
			\item \( yy' + x = 3 x^3 e^{y^2} \)																			% e^{y^2} = C e^{x^2} + 3 \pares{x^2 + 1}
			\item \( 3xy' + xy = y^4 + \frac{y^4}{x} \)																	% \frac{1}{y^3} = Ce^{x} + \frac{1}{x}
			\item \( y' + \pares{x + 3} \cdot e^{x + y} = \frac{2}{x} \)												% e^{-y} = \frac{C}{x^2} + xe^{x}
			\item \( xy' = y + 1 - \pares{y + 1}^2 \sin{x} \)															% \frac{x}{y + 1} = C - \cos{x}
			\item \( \pares{x^3 - 1} y' + \pares{2x^3 + 1} y = 3 x^2 y \ln{y} \)										% \ln{y} = C \pares{x^3 - 1} + x
			\item \( 2xy' - y = y^2 \pares{1 - 3x} \)																	% \frac{x}{y} = C \sqrt{x} + x^2 - x
			\item \( 4y' \tan{x} + 2y = y^3 \sec{x} \)																	% \frac{2}{y^2} = C \sin{x} + \cos{x}
			\item \( 3 \pares{xy^2 y' \ln{x} - 1} = y^3 + x \ln{x} + x \)												% y^3 = C \ln{x} + x + 3
			\item \( y' \tan{y} + \tan{x} = 2 \sec{x} \cos{y} \)														% \sec{y} = C \cos{x} + 2 \sin{x}
			\item \( x^2 y' + \frac{x^2y + 2y^2}{x + 2} = 2y^2 \)														% \frac{1}{y} = C \pares{x + 2} + \frac{1}{x}
			\item \( x y' + y \ln{y} = \frac{y}{x\ln{x}} \pares{x\ln{y} - 1} \)											% x\ln{y} = C \ln{x} + 1
			\item \( 2x^2 y' + 4y^3 \ln{x} = xy \pares{\ln{x} + 1} \)													% \frac{x}{y^2} = \frac{C}{\ln{x}} + 2 \ln{x}
			\item \( 2y' \sin{x} + 2 \cos^2{y} = \sec{x} \sin{2y} \)													% \tan{y} = C \tan{x} + \sec{x}
			\item \( xy' \ln{x} + y \pares{\ln{x} + 1} = xy^2 \)														% \frac{1}{y} = C x \ln{x} + x
			\item \( xy' \ln{x} = xy \ln^2{x} + y\ln{y} \)																% \ln{y} = C \ln{x} + x \ln{x}
			\item \( 2y' \sin{x} + y \sec{x} = 4y^3 \sin^3{x} \)														% \frac{1}{y^2} = C \tan{x} + \sin{2x}
			\item \( 2xy' + y \pares{x + 1} = y^3 \pares{2x + 1} e^{-x} \)												% \frac{1}{y^2} = C xe^{x} + e^{-x}
			\itemstar \( x y' \pares{y + 1} + 2 e^{-y} \ln{x} = 2y + e^{-y} \)											% ye^{y} = C x^2 + \ln{x}
			\itemstar \( y' \pares{\ln{y} + 1} + \ln{x} = \frac{y \ln{y}}{x \ln{x}} \)									% y \ln{y} = C \ln{x} + x\ln{x}
			\itemstar \( x y' + y = \pares{x + 1}e^{x y} - \frac{1}{x + 1} \)											% e^{-xy} = C \pares{x + 1} - x^2 + 1
			\itemstar \( x^2 y' \pares{1 - y} + \pares{x + 2} e^{y} = xy \pares{x + 1} \)								% ye^{-y} = C xe^{x} + \frac{1}{x}
			
		\end{enumtasks}
	\end{multicols}

	\begin{enumtasks}

		\label{firstorder:to_linear2}
		\item \( y' \pares{x + 1} + y + 1 + \pares{xy + x + y + 1}^2 = 0 \)												% \frac{1}{y + 1} = C \pares{x + 1} + x^2 - 1
		\item \( 2x^2 yy' + xy^2 + \sin{x} = x y^2 \pares{x \cot{x} - 1} \)												% x^2 y^2 = C\sin{x} - x \sin{x}
		\item \( y' \pares{x^4 + 1} + 4x^3 y = y^2 \pares{x^3 - x^4 - 1} e^{4x} \)										% \frac{4}{y} = C \pares{x^4 + 1} + e^{4x}
		\itemstar \( xy' \pares{x - 1} = \pares{x + 1} \cdot \pares{x \sqrt{y} + y} + 4x \sqrt{y} \)					% \sqrt{y} = \frac{C \pares{1 - x}}{\sqrt{x}} + x
		\itemstar \( \pares{2 xy^2 + y'} \cdot \ln{\pares{x^2 + 1}} + 2xy^2 + \frac{2xy}{x^2 + 1} = 0 \)				% \frac{1}{y} = C \ln{\pares{x^2 + 1}} + x^2 + 1
		\itemstar \( 2y' \pares{y + 1} \arctan{x} - 1 = 2x \arctan{x} + \frac{\pares{y + 1}^2}{x^2 + 1} \)				% \pares{y + 1}^2 = C \arctan{x} + x^2 + 1
		\itemstar \( xy' \sec^2{y} + \pares{x \tan{x} + 1} \tan{y} = \pares{2 x \tan{x} - 1} \sec{x} \)					% \tan{y} = \frac{C \cos{x}}{x} + \sec{x}
		\itemstar \( \pares{xy' + y} \arctan{y} = \frac{1 - x^2}{\pares{x^2 + 1}^2} - \frac{xyy'}{y^2 + 1} \)			% y \arctan{y} = \frac{C}{x} + \frac{1}{x^2 + 1}

	\end{enumtasks}

	% \pagebreak

	Для следующих уравнений Риккати построить общее решение:
	\begin{enumtasks}

		\label{firstorder:to_linear_riccati}
		\item \( xy' = \pares{x + y}^2 - 2x - y \) 																		% y = \frac{1}{Cx + 1} - x
		\item \( xy' + y \pares{2x^3 + 1} = -x \pares{xy^2 + x^3 + 2} \) 												% xy = \frac{1}{C + x} - x^2
		\item \( y' + 2 = x + y^2 \pares{x - 1} + y \pares{2x - 3} \) 													% y = \frac{1}{C e^{x} + x} - 1
		\item \( xy' - x^2 y^2 = y \pares{2x^4 - 1} + x^6 - 3x^2 \) 													% xy = \frac{1}{C - x} - x^3
		\item \( y' \pares{x + 1} + x \pares{3x + 2 - 2x^3} = 2 y^2 + y \pares{4x^2 - 1} \) 							% y = \frac{1}{C \pares{x + 1} + 2} - x^2
		\item \( \pares{y' - 1} \cos{x} + x^2 + y^2 = x \sin{x} + y \pares{2x - \sin{x}} \) 							% y = \frac{\cos{x}}{C + x} + x
		\itemstar \( y' = y^2 e^{-x} + 3y + e^{x} \) 																	% y = \frac{e^{x}}{C - x} - e^{x}
		\itemstar \( xy' + 1 = y - 2xy^2 + \pares{1 - 4xy - 2x \ln{x}} \ln{x}, ~ y_p = A \ln{bx} \)						% y = \frac{x}{C + x^2} - \ln{x}
		\itemstar \( xy' \ln{x} + y + 2 = 2x\pares{y + 2}^2 \pares{1 - \ln{x}} \)										% y = \frac{1}{C \ln{x} + 2x} + 2
		\itemstar \( y' + \pares{y^2 + 1} e^{x} = y \pares{2e^{x} - 1} + 1 \) 											% \pares{y - 1} e^{x} = \frac{1}{C + x}
		\itemstar \( xy' + y \pares{x + 1} = x^2 \pares{y - e^{-x}}^2 + e^{-x} \) 										% xy = \frac{1}{Ce^{x} + 1} + xe^{-x}
		\itemstar \( y' \tan{x} + y^2 e^{x} = 2ye^{x} \tan{x} + y \sec^2{x} - e^{x} \tan^2{x} \)						% y = \frac{\tan{x}}{C + e^{x}} + \tan{x}
		\itemstar \( 2xy' + y + 3 x^2 y^{2} - 2e^{x} = 4 x \pares{3xy - 3xe^{x} + 1} e^{x}, ~ y_p = Ae^{x} \)			% y = \frac{1}{C \sqrt{x} + x^2} + 2e^{x}
		\itemstar \( xy' \ln{x} + y + y^2 = 2 \pares{y + 1} \ln{x} - \ln^2{x} \) 										% y = \frac{1}{C \ln{x} - 1} + \ln{x}
		\itemstar \( y' e^{x} \pares{x^2 - 1} + 2xye^{x} = \pares{y^2 - 2ye^{x} + 2e^{2x}} \pares{x^2 + 2 x - 1} \)		% y = \frac{e^{x}}{C \pares{x^2 - 1}e^{x} + 1} + e^{x}

	\end{enumtasks}
