% Boundary Problems
\subsection*{Краевые задачи, метод подстановки}
	\begin{enumsols}

		% \label{sol:bvp_bvp:constcoeffs_simple}
		\item \( y = 0 \); \sfill % \( y'' = 0, ~ y(0) = 0, ~ y(1) = 0 \)		% y = 0
		\item \( y = x \); \sfill % \( y'' = 0, ~ y(0) = 0, ~ y(1) = 1 \)		% y = x
		\item \( y = e^{x} - 1 \); \sfill % \( y'' - y' = 0, ~ y(0) = 0, ~ y \pares{\ln{2}} = 1 \)		% y = e^{x} -1
		\item \( y = 2 e^{x} - e^{2 x} \); \sfill % \( y'' - 3 y' + 2 y = 0, ~ y(0) = 1, ~ y \pares{\ln{2}} = 0 \)		% y = 2 \cdot e^{x} - e^{2 x}
		\item \( y = e^{3 x} + e^{x} \); \sfill % \( y'' - 4 y' + 3 y = 0, ~ y(0) = 2, ~ y \pares{\ln{2}} = 10 \)		% y = e^{3 x} + e^{x}
		\item \( y = e^{2 x} - 3 e^{- x} \); \sfill % \( y'' - y' - 2 y = 0, ~ y(0) = -2, ~ y \pares{\ln{3}} = 8 \)		% y = e^{2 x} -3 \cdot e^{- x}
		\item \( y = e^{3 x} - 9 e^{- 2 x} \); \sfill % \( y'' - y' - 6 y = 0, ~ y(0) = -8, ~ y \pares{\ln{3}} = 26 \)		% y = e^{3 x} -9 \cdot e^{- 2 x}
		\item \( y = e^{2 x} \pares{1 - x} \); \sfill % \( y'' - 4 y' + 4 y = 0, ~ y(0) = 1, ~ y(1) = 0 \)		% y = e^{2 x} - x e^{2 x}
		\item \( y = e^{x} - 5 e^{- x} \); \sfill % \( y'' - y = 0, ~ y(0) = -4, ~ y \pares{\ln{5}} = 4 \)		% y = e^{x} -5 \cdot e^{- x}
		\item \( y = 4 \sinh{2x} - 2 e^{-2x} \); \sfill % \( y'' - 4 y = 0, ~ y(0) = -2, ~ y \pares{\ln{2}} = 7 \)		% y = 2 \cdot e^{2 x} -4 \cdot e^{- 2 x}
		\item \( y = \cos{x} \); \sfill % \( y'' + y = 0, ~ y(0) = 1, ~ y \pares{\frac{\pi}{2}} = 0 \)		% y = \cos{x}
		\item \( y = 2 \cos{2 x} \); \sfill % \( y'' + 4 y = 0, ~ y(0) = 2, ~ y \pares{\frac{\pi}{3}} = -1 \)		% y = 2 \cdot \cos{2 x}
		\item \( y = 2 e^{x} \pares{\cos{x} + \sin{x}} \); \sfill % \( y'' - 2 y' + 2 y = 0, ~ y(0) = 2, ~ y \pares{\pi} = - 2 e^{\pi} \)		% y = 2 \cdot e^{x} \cos{x} + 2 \cdot e^{x} \sin{x}
		\item \( y = e^{x} \pares{\cos{2 x} + \sin{2 x}} \); \sfill % \( y'' - 2 y' + 5 y = 0, ~ y(0) = 1, ~ y \pares{\pi} = e^{\pi} \)		% y = e^{x} \cos{2 x} + e^{x} \sin{2 x}
		\item \( y = \pares{x - 1}^2 \); \sfill % \( y'' = 2, ~ y'(0) = -2, ~ y'(1) = 0 \)		% y = 1 -2 \cdot x + x^{2}
		
		\label{sol:bvp_bvp:constcoeffs_nonhmg}
		\item \( y = e^{x} + x \); \sfill % \( y'' - y' = -1, ~ y(-1) = -1 + e^{-1}, ~ y'(1) = 1 + e \)		% y = -2 + e^{x} + x + 2
		\item \( y = e^{x} \pares{x + 1} - 2 e^{- x} \); \sfill % \( y'' - y = 2 e^{x}, ~ y(0) = -1, ~ y' \pares{\ln{2}} = \ln{4} + 5 \)		% y = e^{x} -2 \cdot e^{- x} + x e^{x}
		\item \( y = 1 - \sin{x} \); \sfill % \( y'' - 2 y' + 2 y = 2 - \sin{x} + 2 \cos{x}, ~ y'(-1) = y'(1) = - \cos{1} \)		% y = 1 - \sin{x}
		\item \( y = \sin{2 x} + e^{4 x} \); \sfill % \( y'' + 4 y = 20 e^{4 x}, ~ 2 y(0) - y'(0) = -4, ~ y \pares{\frac{\pi}{4}} - y' \pares{\frac{\pi}{4}} = 1 - 3 e^{\pi} \)		% y = \sin{2 x} + e^{4 x}
		\item \( y = \frac{2}{\pi} \cdot \cos{2 x} - \frac{1}{\pi} \cdot \sin{2 x} + \frac{\pi^2}{x} \); \sfill % \( y'' + 4 y = \frac{2\pi^2}{x^3} \cdot \pares{2x^2 + 1}, ~ y \pares{-\pi} + y' \pares{-\pi} = - \pi - 1, ~ y \pares{\pi} - y' \pares{\pi} = \frac{4}{\pi} + 1 + \pi \)		% y = 2/pi \cdot \cos{2 x} -1/pi \cdot \sin{2 x} + \frac{\pi^{2}}{x}

		\label{sol:bvp_bvp:linear}
		\item \( y = x + \frac{1}{x} \); \sfill % \( x^2 y'' + xy' - y = 0, ~ y(-1) = -2, ~ y(1) = 2 \) % y = x + \frac{1}{x}
		\item \( y = x^2 - x + 1 \); \sfill % \( y'' x \pares{x - 2} + 2y = 2y' \pares{x - 1}, ~ y(0) = 1, ~ y(1) = 1 \) % y = x^2 - x + 1
		\item \( y = e^{x} - x \); \sfill % \( y'' \pares{x - 1} - xy' + y = 0, ~ y(0) = 1, ~ y' \pares{\ln{2}} = 1 \) % y = - x + e^{x}
		\item \( y = 3 x e^{- x} - e^{x} \); \sfill % \( y'' \pares{2x - 1} - 2y' = y \pares{2x - 3}, ~ y'(0) = 2, ~ y \pares{\ln{3}} = \ln{3} - 3 \) % y = 3 x e^{- x} - e^{x}
		\item \( y = \cos{x} + 4 \tan{x} - \sec{x} \); \sfill % \( y'' + 2 \cos{x} = y' \tan{x} + y \sec^2{x}, ~ y(0) = 0, ~ y'\pares{\pi} = 4 \) % y = \cos{x} + 4 \tan{x} - \sec{x}
		\item \( y = \sin{2x} - x + 1 \); \sfill % \( y'' \pares{2x \cot{2x} - 1}= 4 \pares{y - xy' - 1}, ~ y'(0) = 1, ~ y\pares{\pi} = 1 - \pi \) % y = \sin{2x} - x + 1
		
		\label{sol:bvp_bvp:linear_hard}
		\item \( y = 2 \cosh{x} - x \); \sfill % \( y'' \pares{x - 1} - xy' + y = 2xe^{-x}, ~ y(0) + y'(1) = 1 + 2 \sinh{1}, ~ y(1) - y'(1) = \frac{2}{e} \) % y = e^{x} + e^{- x} - x
		\item \( y = 2 \ln{x} + e^{- x} + 1 \); \sfill % \( x y'' \pares{x \ln{x} + 1} + y' \pares{x^2 \ln{x} + 1} = \pares{y - 1} \pares{x - 1}, ~ y(1) + y'(1) = 3, ~ y(1) - y'(2) = \frac{1 + e}{e^2} \) % y = 2 \ln{x} + 1 + e^{- x}
		\item \( y = x^2 + x + 2 \arctan{x} \); \sfill % \( \syst{&\pares{x^2 + 1}^2 \pares{y'' - 2} \arctan{x} + x \pares{x^2 + 1} \pares{y'' - 2} + 2xy = 2x^2 \pares{y' - x}, \\ &y(0) + 2y(1) = \pi + 4, ~ y'(1) - y'(0) = 1} \) % y = x^{2} + x + 2 \arctan{x}
		\item \( y = 2 x \ln{x} + x + e^{x} \); \sfill % \( \syst{&x^2 \ln{x} \pares{y'' - y'} - x \ln{x} \pares{y'' - y} - xy'' + y' + \pares{x - 1} y = x^2 - x + 1, \\ &y'(1) - y(1) = 2, ~ 2y'(1) + 2y'(2) - y(2) = 2e + e^2 + 10} \) % y = 2 x \ln{x} + x + e^{x}

		\label{sol:bvp_bvp:nonlinear}
		\item \( y^2 = 4 \ln{x} \); \sfill % \( xyy'' + xy'^2 + yy' = 0, ~ y(1) = 0, ~ y(2) \cdot y'(2) = 1 \) % y^2 = 4 \ln{x}
		\item \( e^{- y} = \pares{x + 1}^2 \); \sfill % \( y'' - y'^2 = \frac{y'}{x + 1}, ~ y(0) - y'(0) = 2, ~ y'(1) = -1 \) % e^{- y} = \pares{x + 1}^2
		\item \( y \sinh{y} = x \); \sfill % \( y'^2 \pares{y \tanh{y} + 2} = \pares{y' - y''} \cdot \pares{y + \tanh{y}}, ~ y(0) = 0, ~ y(\sinh{1}) = 1 \) % y \sinh{y} = x
		\item \( x^2 \ln{y} = x^2 -  e^2 \ln{x} \); \sfill % \( x \pares{2 \ln{x} - 1} \cdot \pares{y'^2 - yy''} = yy' \cdot \pares{6 \ln{x} - 5}, ~ y(1) = e, ~ y(e) = 1 \) % x^2 \ln{y} = x^2 -  e^2 \ln{x}
		\item \( y = 1  \); \sfill % \( 2yy' \pares{\cos^2{x} + 1} + \pares{yy'' + y'^2} \sin{2x} = 0, ~ y(0) = 0, ~ y \pares{\frac{\pi}{2}} = 1 \) % y = 1 
		\item \( \tan{y} = C_1 \tan{x} + C_2 \); \sfill % \( y'' + 2y'^2 \tan{y} = 2y' \tan{x}, ~ y\pares{\frac{\pi}{4}} = \frac{\pi}{4}, ~ y'(\pi) = 0 \) % \tan{y} = C_1 \tan{x} + C_2
		
		\label{sol:bvp_bvp:nonlinear_hard}
		\item \( e^y = (e - 1) \cdot x e^x + 1 \); \sfill % \( y'' + y'^2 - y' = \frac{y'}{x + 1}, ~ y'(-1) - y(-1) = 1, ~ y(0) + y'(0) = e - 1 \) % e^y = (e - 1) \cdot x e^x + 1
		\item \( \sin{y} = 1 - \ln{x} \); \sfill % \( xy'' + y' = xy'^2 \tan{y}, ~ y'(1) \cdot \cos{y(1)} = -1, ~ y(e) = 0 \) % \sin{y} = 1 - \ln{x}
		\item \( y^2 = 4 \arctan{x} - 2 \); \sfill % \( 2xyy' + \pares{x^2 + 1} \cdot \pares{yy'' + y'^2} = 0, ~ y(0) \cdot y'(0) = 2, ~ y^2(1) + 2y(0) \cdot y'(1) = \pi \) % y^2 = 4 \arctan{x} - 2
		\item \( x e^{y - x} = 1 \); \sfill % \( xy'^2 + xy'' + 2x = y' \pares{3x - 2} + 3, ~ y(1) = 1, ~ y(e) = e - 1 \) % x e^{y - x} = 1
	
	\end{enumsols}

% Linear Greens
\subsection*{Функции Грина}

	\begin{enumsolsfull}

		\label{sol:bvp_green:int_factor}
		\item \( w = x, ~ \mu = \frac{1}{x}, ~ \pares{xu', v'} + \pares{\frac{u}{x}, v} = 0, ~ u = x \); % \( x^2 u'' + xu' - u = 0, ~ u(-1) = -1, ~ u(1) = 1 \) % u = x;
		\item \( w = x, ~ \mu = \frac{e^x}{x^2}, ~ \pares{\frac{e^x}{x} u', v'} + \pares{\frac{e^x}{x^2} u, v} = 0, ~ u = x \); % \( xu'' + \pares{x - 1} u' - u = -1, ~ u(0) = 0, ~ u(1) = 1 \) % u = x;
		\item \( w = x + e^x, ~ \mu = \frac{1}{\pares{2x - 1}^2}, ~ \pares{\frac{u'}{2x - 1}, v'} + \pares{\frac{2x - 3}{\pares{2x - 1}^2} u, v} = 0, ~ u = x + e^x \); % \( \pares{2x - 1} u'' - 2u' - \pares{2x - 3} u = 3x - 2x^2 - 2, ~ u(-1) = \frac{1}{e} - 1, ~ u(1) = 1 + e \) % u = x + e^x;
		\item \( w = 1, ~ \mu = \frac{1}{x^4}, ~ \pares{\frac{u'}{x^2}, v'} - 2\pares{\frac{u}{x^4}, v} = -\pares{\frac{2}{x^4}, v}, ~ u = x^2 - x + 1 \); % \( x^2 u'' = 2 \pares{xu' - u + 1}, ~ u(0) = 1, ~ u(1) = 1 \) % u = x^2 - x + 1;
		\item \( \begin{aligned} &w = 2 - x, ~ \mu = \frac{1}{x^2 \pares{x - 4}^2}, \\ &\pares{\frac{u'}{x\pares{x - 4}}, v'} - 2\pares{\frac{u}{x^2 \pares{x - 4}^2}, v} = 4 \pares{\frac{1}{x^2 \pares{x - 4}^2}, v}, ~ u = x^2 - 2x + 2 \end{aligned} \); % \( x \pares{x - 4} u'' - 2 \pares{x - 2} u' + 2u = - 4, ~ u(0) = 2, ~ u(1) = 1 \) % u = x^2 - 2x + 2;
		\item \( \begin{aligned} &w = x + 2, ~ \mu = \frac{x - 1}{x^2}, \\ &\pares{\frac{\pares{x-1}^2}{x} u', v'} + \pares{\frac{\pares{x-1}}{x^2} u, v} = \pares{\pares{3 + \frac{1}{x^2}} \pares{1 - x}, v}, ~ u = x^2 + x + 1 \end{aligned} \); % \( x \pares{x - 1} u'' + \pares{x + 1} u' - u = 3x^2, ~ u(-1) = 1, ~ u(1) = 3 \) % u = x^2 + x + 1;
		\item \( \begin{aligned} &w = \cos{x}, ~ \mu = \cosec^3{x}, \\ &\pares{u' \cosec^3{x}, v'} - \pares{\pares{2 + \cos{2x}} \cdot u \cosec^5{x}, v} = 0, ~ u = \sin{2x} + \cos{x} \end{aligned} \); % \( u'' - 3u' \cot{x} + \pares{3 \cosec^2{x} - 2} u = 3 \cot{x} \cosec{x}, ~ u(0) = 1, ~ u\pares{\frac{\pi}{2}} = 0 \) % u = \sin{2x} + \cos{x};
		\item \( \begin{aligned} &w = 2x - 1 - e^x, ~ \mu = \frac{e^{-x}}{x^2 \pares{x - 2}^2}, \\ &\pares{\frac{e^{-x}}{x \pares{x-2}} u', v'} - 2 \pares{\frac{e^{-x} \pares{x-1}}{x^2 \pares{x - 2}^2} u, v} = \pares{\frac{e^{-x} \pares{x^2 - 2x + 2}}{x^2 \pares{x - 2}^2}, v}, ~ u = x^2 + x - e^x - 1 \end{aligned} \); % \( x \pares{x - 2} u'' - \pares{x^2 - 2} u' + 2 \pares{x - 1} u = \pares{x - 2}^2, ~ u(0) = -2, ~ u(1) = 1 - e \) % u = x^2 + x - e^x - 1;
		\item \( w = x + 2, ~ \mu = \frac{1}{\pares{xe^x + 1}^2}, ~ \pares{\frac{u'}{xe^x + 1}, v'} - \pares{\frac{e^x}{\pares{xe^x + 1}^2} u, v} = 0, ~ u = x + 2 \); % \( \pares{x e^x + 1} u'' - \pares{x + 1} u' e^x + u e^x = e^x, ~ u(0) = 2, ~ u(1) = 3 \) % u = x + 2;
		\item \( \begin{aligned} &w = x + \ln{x}, ~ \mu = \frac{1}{x^4 \pares{\ln{x} - 1}^2}, \\ &\pares{\frac{u'}{x^2 \pares{\ln{x} - 1}}, v'} - 2 \pares{\frac{\ln{x}}{x^4 \pares{\ln{x} - 1}^2} u, v} = \pares{\frac{2\ln^2{x} - 5 \ln{x} + x + 2}{x^4 \pares{\ln{x} - 1}^2}, v}, ~ u = x \ln{x} + 1 \end{aligned} \); % \( x^2 \pares{\ln{x} - 1} u'' - x \pares{2 \ln{x} - 1} u' + 2 u \ln{x} = 2 \ln{x}, ~ u(1) = 1, ~ u(e) = 1 + e \) % u = x \ln{x} + 1;

	\end{enumsolsfull}

	\begin{enumsols}

		% \label{sol:bvp_green:green_lifting}
		\item \( \mu = 1, ~ y = 1 - x + x e^x \); % \( y'' = \pares{x + 2} e^x, ~ y(0) = 1, ~ y(1) = e \) % y = 1 - x + x e^x
		\item \( \mu = e^{-x}, ~ y = e^x + 1 + x^2 + x \); % \( y'' - y' = 1 - 2 x, ~ y(0) = 2, ~ y(1) = e + 3 \) % y = e^x + 1 + x^2 + x
		\item \( \mu = 1, ~ y = \sinh{x} + x e^x \); % \( y'' - y = 2 e^x, ~ y(0) = 0, ~ y\pares{\ln{2}} = \ln{4} + 3 \) % y = \sinh{x} + x e^x
		\item \( \mu = e^{-3x}, ~ y = \pares{x^2 + 1} \cdot e^x - e^{2x} \); % \( y'' - 3 y' + 2 y = 2 \cdot \pares{1 - x} e^x, ~ y(0) = 0, ~ y(1) = 2e - e^2 \) % y = \pares{x^2 + 1} \cdot e^x - e^{2x}
		% \newline
		\item \( \mu = e^{-2x}, ~ y = x \cdot \pares{e^x + 1} + e^{2x} \); % \( y'' - 2 y' + y = x + e^{2x} - 2, ~ y(0) = 1, ~ y(1) = 1 + e + e^2 \) % y = x \cdot \pares{e^x + 1} + e^{2x}
		\item \( \mu = e^{-x}, ~ y = \pares{x + 1} \cdot e^{2x} \); % \( y'' - y' - 2 y = 3 e^{2x}, ~ y(0) = 1, ~ y\pares{\ln{3}} = 9 \pares{1 + \ln{3}} \) % y = \pares{x + 1} \cdot e^{2x}
		\item \( \mu = 1, ~ y = \pares{x + 1} \cdot \cosh{2x} \); % \( y'' - 4 y = 4 \sinh{2 x}, ~ y(-1) = 3 \cosh{2}, ~ y(1) = 5 \cosh{2} \) % y = \pares{x + 1} \cdot \cosh{2x}
		\item \( \mu = e^{-4x}, ~ y = \pares{x - 1}^2 e^{2x} + x \); % \( y'' - 4 y' + 4 y = 4 x + 2 e^{2x} - 4, ~ y(0) = 1, ~ y'(1) = 1 \) % y = \pares{x - 1}^2 e^{2x} + x
		
		\label{sol:bvp_green:green_lifting_hard}
		\item \( \mu = e^{-2x}, ~ y = e^x - 2x e^x + x \cosh{x} \); % \( y'' - 2 y' + y = 2 \pares{x - 1} e^{-x}, ~ y'(-1) = 2 \cosh{1}, ~ y'(1) = - 2 e \) % y = e^x - 2x e^x + x \cosh{x}
		% \newline
		\item \( \mu = 1, ~ y = \cos{x} + \cosh{x} \); % \( y'' + y = 2 \cosh{x}, ~ y(0) = 2, ~ y\pares{\frac{\pi}{2}} = \cosh{\frac{\pi}{2}} \) % y = \cos{x} + \cosh{x}
		\item \( \mu = 1, ~ y = x \sin{x} - \cos{x} \); % \( y'' + y = 2 \cos{x}, ~ y(0) = -1, ~ y'\pares{\pi} = - \pi \) % y = x \sin{x} - \cos{x}
		\item \( \mu = e^{-2x}, ~ y = e^x \cos{x} + x + 1 \); % \( y'' = 2 \pares{y' - y + x}, ~ y(0) = 2, ~ y'\pares{\pi} = 1 - e^{\pi} \) % y = e^x \cos{x} + x + 1
		\item \( \mu = e^{-2x}, ~ y = e^x \cos{2x} - \sin{x} + 2 \cos{x} \); % \( y'' - 2 y' + 5 y = 10 \cos{x}, ~ y(0) + y'(0) = 3, ~ y\pares{\pi} = e^{\pi} - 2 \) % y = e^x \cos{2x} - \sin{x} + 2 \cos{x}
		\item \( \mu = e^{-2x}, ~ y = \pares{\cos{2x} + \sin{2 x} + x} e^x \); % \( y'' - 2 y' + 5 y = 4 x e^x, ~ y(0) + y'(0) = 5, ~ y\pares{\pi} = \pares{1 + \pi} e^{\pi} \) % y = \pares{\cos{2x} + \sin{2 x} + x} e^x
		\item \( \mu = e^{2x}, ~ y = \pares{\cos{x} + 1} e^{- x} \); % \( y'' + 2 y' + 2 y = e^{-x}, ~ y'(0) = -2, ~ y\pares{\pi} - y'\pares{\pi} = 0 \) % y = \pares{\cos{x} + 1} e^{- x}
		\item \( \mu = e^{4x}, ~ y = \pares{\sin{x} - \cos{x}} \cdot e^{-2x} + xe^x \); % \( y'' + 4 y' + 5 y = 2 \cdot \pares{5x + 3} \cdot e^x, ~ 2y'(0) - y(0) = 9, ~ y\pares{\pi} = e^{-2\pi} + \pi e^{\pi} \) % y = e^{-2x} \sin{x} - e^{-2x} \cos{x} + xe^x
		
		% \newline
		\item \( \mu = e^{-2x}, ~ y = e^{-x} \sin{2x} + x^2 \); % \( y'' + 2 y' + 5 y = 5 x^2 + 4 x + 2, ~ 2y'(0) - y(0) = 4, ~ y\pares{\frac{\pi}{4}} + y'\pares{\frac{\pi}{4}} = \pares{\frac{\pi}{4}}^2 + \frac{\pi}{2} \) % y = e^{-x} \sin{2x} + x^2
		
		\item \( \mu = e^{6x}, ~ y = e^{-x} \sin{2x} + x^2 \); % \( y'' + 6 y' + 13 y = 13 x + 6, ~ y(0) + y'(0) = -3, ~ y'\pares{\pi} = 1 - 5e^{-3 \pi} \) % y = e^{-3x} \cos{2x} - e^{-3x} \sin{2x} + x
		% \newline
		\item \( \mu = 1, ~ y = \cos{2 x} - \sin{6 x} + \tan{x} \); % \( y'' + 4 y = 32 \sin{6 x} + 2 \tan^{3}{x} + 6 \tan{x}, ~ y(0) - y'(0) = 6, ~ 2 y\pares{\frac{\pi}{4}} + y'\pares{\frac{\pi}{4}} = 4 \) % y = \cos{2 x} - \sin{6 x} + \tan{x}
		\item \( \mu = e^{-6x}, ~ y = 2 \cdot e^{3 x} \sin{2 x} + \pares{2\sin{x} - \cos{x}} \cdot e^{-x} \); % \( \syst{&y'' - 6 y' + 13 y = 5 \cdot \pares{6 \sin{x} - 7 \cos{x}} e^{- x}, \\ &y\pares{-\pi} + 2 y'\pares{-\pi} = 8 e^{-3\pi} - 5 e^{\pi}, ~ y\pares{\pi} - y'\pares{\pi} = 4 \cdot \pares{e^{-\pi} - e^{3\pi}}} \) % y = 2 \cdot e^{3 x} \sin{2 x} + 2 e^{- x} \sin{x} - e^{- x} \cos{x}

		\label{sol:bvp_green:green_linear}
		\item \( \mu = \frac{1}{x^4}, ~ y = x^{3} + 1 - \frac{2}{x} \); % \( x^2 y'' - xy' = 3 \pares{y - 1}, ~ y(-1) = 2, ~ y'(1) = 5 \) % \mu = \frac{1}{x^4}, ~ y = x^{3} + 1 - \frac{2}{x}
		\item \( \mu = \frac{1}{x}, ~ y = x + 1 + \frac{1}{x} - \frac{1}{x^2} \); % \( x^3 y'' + 2 x^2 y' = 2 \pares{xy - x - 1}, ~ y(-1) = -2, ~ y(1) = 2 \) % \mu = \frac{1}{x}, ~ y = x + 1 + \frac{1}{x} - \frac{1}{x^2}
		\item \( \mu = \frac{1 + x}{x^2}, ~ y = x^2 + x - 1 + \frac{1}{x + 1} \); % \( x \pares{x + 1} y'' + \pares{x - 1} y' = y + 3x^2, ~ y'(0) = -1, ~ y(1) = 2 \) % \mu = \frac{1 + x}{x^2}, ~ y = x^2 + x - 1 + \frac{1}{x + 1}
		\item \( \mu = \frac{1}{x^2 \pares{\ln{x} - 1}^2}, ~ y = x^2 + x - 1 \); % \( x^2 \pares{\ln{x} - 1} y'' - x y' + y = \pares{2\ln{x} - 3} \cdot x^2 - 1, ~ y'(0) = 1, ~ y'(1) = 3 \) % \mu = \frac{1}{x^2 \pares{\ln{x} - 1}^2}, ~ y = x^2 + x - 1
		\item \( \mu = \frac{xe^{-x}}{\pares{x + 1}^2}, ~ y = - e^{x} + 1 + \frac{1}{x} \); % \( x \pares{x + 1} y'' - \pares{x^2 - 2}y' = \pares{x + 2} \pares{y - 1}, ~ y(-1) = -\frac{1}{e}, ~ y(1) + y'(1) = 1 - 2e \) % \mu = \frac{xe^{-x}}{\pares{x + 1}^2}, ~ y = - e^{x} + 1 + \frac{1}{x}
		\item \( \mu = \frac{e^{-x}}{1 - 2x}. ~ y = x^2 + e^{2x} \); % \( \pares{1 - 2x} y'' + 4xy' - 4y = \pares{1 - 2x}^2 + 1, ~ y(-1) = 1 + \frac{1}{e^2}, ~ y'(0) - y(0) = 1 \) % \mu = \frac{e^{-x}}{1 - 2x}. ~ y = x^2 + e^{2x}
		
		\label{sol:bvp_green:green_linear_hard}
		\item \( \mu = \sec^3{x}, ~ y = \cos{x} + 1 \); % \( \syst{&2 y'' \cos^2{x} + 3y' \sin{2x} + 2 \pares{2 - \cos{2x}} y = 4 - 2 \cos{2x}, \\ &y'(0) = 0, ~ y \pares{\frac{\pi}{2}} - y' \pares{\frac{\pi}{2}} = 2} \) % \mu = \sec^3{x}, ~ y = \cos{x} + 1
		\item \( \mu = \frac{\sec{x}}{\pares{x - \tan{x}}^2}, ~ y = x^2 + x + \sin{x} \); % \( \syst{&\pares{x - \tan{x}} y'' + \pares{x y' - y} \tan{x} = \pares{x^2 - 2} \tan{x} + 2x, \\ &y(0) - y'(0) = -2, ~ y\pares{\frac{\pi}{2}} - y'\pares{\frac{\pi}{2}} = \frac{\pi^2}{4} - \frac{\pi}{2}} \) % \mu = \frac{\sec{x}}{\pares{x - \tan{x}}^2}, ~ y = x^2 + x + \sin{x}
		\item \( \mu = \frac{1}{\pares{2x - 1}^2}, ~ y = x + e^{x} \); % \( \syst{&\pares{2 x - 1} y'' - 2 y' + \pares{3 - 2x} y = 3x - 2x^2 - 2, \\ &2y\pares{-\ln{2}} + 2y' \pares{-\ln{2}} = 4 - 2\ln{2}, ~ y'(0) - y(0) = 1} \) % \mu = \frac{1}{\pares{2x - 1}^2}, ~ y = x + e^{x}
		
		% \newline
		\item \( \mu = \frac{1}{\pares{\ln{x} + 1}^2}, ~ y = x + 2 \ln{x} + \frac{4}{x} \); % \( \syst{&x^2 \pares{\ln{x} + 1} y'' + x \pares{2 \ln{x} + 1} y' - y = 2x \ln{x}, \\ &y(1) + 2y'(1) = 3, ~ 2y(2) - y'(2) = 4 \ln{2} + 7} \) % \mu = \frac{1}{\pares{\ln{x} + 1}^2}, ~ y = x + 2 \ln{x} + \frac{4}{x}

	\end{enumsols}

% Sturm-Liouville
% \subsection*{Задачи Штурма-Лиувилля}

