\subsection{Задачи}

	Построить общее решение следующих линейных неоднородных систем уравнений с постоянными коэффициентами:
	\begin{multicols}{2}
		\begin{enumtasks}

			% \item \( \syst{\dot{x} &= ax + by, \\ \dot{y} &= ax + by} \) % \( x = C_1 + C_2 + , ~ y = C_1 + C_2 + \)

			\label{linsys_nonhmg:quasipolys}
			\item \( \syst{\dot{x} &= t - x - 2y, \\ \dot{y} &= y - t + 1} \) % \( x = C_1 e^{-t} + C_2e^t - t + 1, ~ y = t - C_2 e^{t} \)
			\item \( \syst{\dot{x} &= 3x + y, \\ \dot{y} &= t - 4x - y - 3} \) % \( x = C_1e^{t} + C_2 \pares{t+1} e^{t} + t - 1 , ~ y = 4 - 2C_1 e^{t} - C_2 \pares{2t + 1} e^{t} - 3t \)
			\item \( \syst{\dot{x} &= y + 2t + 1, \\ \dot{y} &= t^2 - x - 2y} \) % \( x = t^2 + 2 - C_1e^{-t} - C_2 \pares{t-2} e^{-t} , ~ y = C_1e^{-t} + C_2 \pares{t - 3}e^{-t} - 1 \)
			\item \( \syst{\dot{x} &= 9y - 4x - 5e^{t} - 18t + 3, \\ \dot{y} &= 8y - 4x - 4e^{t} - 16t + 6} \) % \( x = 3C_1e^{2t} + C_2 \pares{3t + 1}e^{2t} + 3 - e^{t}, ~ y = 2C_1e^{2t} + C_2 \pares{1 + 2t} e^{2t} + 2t + 1 \)
			\item \( \syst{\dot{x} &= 2\sin{t} - x - 8y + 8, \\ \dot{y} &= 3y - 3} \) % \( x = C_1e^{-t} + 2C_2 e^{3t} + \sin{t} - \cos{t}, ~ y = 1 - C_2 e^{3t} \)
			\item \( \syst{\dot{x} &= x - 2y + 2\cos{t}, \\ \dot{y} &= x - y + \cos{t} - 3\sin{t}} \) % \( x = C_1 \pares{\cos{t} + \sin{t}} - 2C_2 \sin{t} + 2\sin{t} - 2t \cos{t}, ~ y = C_1\sin{t} + C_2 \pares{\cos{t} - \sin{t}} - \pares{t-1} \pares{\sin{t} + \cos{t}} \)
			\item \( \syst{\dot{x} &= 3x - 4y + 4e^{-t} - 3, \\ \dot{y} &= 2x - y - 2} \) % \( x = C_1 e^{t} \pares{\sin{2t} + \cos{2t}} - 2C_2 e^{t} \sin{2t} + 1, ~ y = C_1 e^{t} \sin{2t}  + C_2 e^{t} \pares{\cos{2t} - \sin{2t}} + e^{-t} \)
			\item \( \syst{\dot{x} &= 2y - x + 3\pares{t + 1} e^{2t} - 2t, \\ \dot{y} &= \pares{2t - 7} e^{2t} + 5t + 1 - 2x - 5y} \) % \( x = 2C_1 e^{-3t} + C_2 \pares{2t + 1} e^{-3t} + te^{2t}, ~ y = t - 2C_1 e^{-3t} - 2C_2t e^{-3t} - e^{2t} \)
			\item \( \syst{\dot{x} &= 5x - 3y + 5 \sin{t} - \cos{t}, \\ \dot{y} &= 6x - 4y + 6\sin{t}} \) % \( x = C_1 e^{2t} + C_2 e^{-t} + \sin{t}, ~ y = C_1 e^{2t} + 2C_2e^{-t} \)
			\item \( \syst{\dot{x} &= x - y - e^{t} \cos{t}, \\ \dot{y} &= x + y + e^{t} \sin{t}} \) % \( x = C_1 e^{t} \sin{t} + C_2 e^{t} \cos{t} + e^{t} \sin{t}, ~ y = -C_1 e^{t} \cos{t} + C_2 e^{t} \sin{t} \)

			\label{linsys_nonhmg:general}
			\item \( \syst{\dot{x} &= y - x - \pares{\sin{t} + \sec{t}} \tan{t}, \\ \dot{y} &= 3y - 4x + 3\cos{t} - 4\sec{t} + \sin{t}} \) % \( x = C_1e^{t} + C_2 \pares{1-t} e^{t} + \sec{t}, ~ y = 2C_1 e^{t} + C_2 \pares{1 - 2t} e^t + \cos{t} \)
			\item \( \syst{\dot{x} &= x - y + 1 + e^{-2t} \ln{t}, \\ \dot{y} &= \frac{e^{-2t}}{t} - 2y} \) % \( x = C_1e^{-2t} + C_2e^{t} + 1, ~ y = 3C_1e^{-2t} - e^{-2t} \ln{t} \)
			\item \( \syst{\dot{x} &= \frac{e^t}{t} - y, \\ \dot{y} &= 4x - \frac{e^t}{t^3} \pares{4t^2 - t + 2}} \) % \( x = C_1 \cos{2t} - C_2 \sin{2t} - \frac{e^t}{t} , ~ y = 2 C_1 \sin{2t} + 2C_2 \cos{2t} - \frac{e^t}{t^2} \)
			\item \( \syst{\dot{x} &= 3x + y - 2 + \pares{3t - 2} \ln{t}, \\ \dot{y} &= \frac{1}{t} - 6x - 2y - 2\pares{3t - 1} \ln{t}} \) % \( x = C_1 - C_2 e^{t} + t \ln{t}, ~ y = -3C_1 + 2C_2 e^{t} - \ln{t} \)
			\item \( \syst{\dot{x} &= x + y + \pares{t-1}^2 - t \ln{t} - 1, \\ \dot{y} &= \pares{1+t} \pares{\ln{t} - t + 1} - x - y} \) % \( x = C_1 + C_2 \pares{2t + 1} + t^2, ~ y = -C_1 - C_2 \pares{2t - 1} - t \ln{t} \)
			\itemstar \( \syst{\dot{x} &= \arctan{t} - x - y - t - 1, \\ \dot{y} &= x - 3y + t + \frac{1}{t^2 + 1} + 3\arctan{t}} \) % \( x = C_1e^{-2t} - \pares{t + 1} C_2 e^{-2t} + t, ~ y = C_1 e^{-2t} - C_2t e^{-2t} + \arctan{t} \)
			
			% \item \( \syst{\dot{x} &= ax + by + cz, \\ \dot{y} &= ax + by + cz, \\ \dot{z} &= ax + by + cz} \) % \( x = C_1 + C_2 + C_3 +, ~ y = C_1 + C_2 + C_3 +, ~ z = C_1 + C_2 + C_3 + \)

			\label{linsys_nonhmg:hard}
			\itemstar \( \syst{\dot{x} &= 2y - 3t^2, \\ \dot{y} &= z + 2 \ln{t}, \\ \dot{z} &= -\frac{2}{t}} \) % \( x = C_1 + 2C_2t + C_3t^2 - 3t^2, ~ y = C_2 + C_3t, ~ z = C_3 + 2 \ln{t} \)
			\itemstar \( \syst{\dot{x} &= x - 2t e^t, \\ \dot{y} &= y + z + \sin{t} - 1, \\ \dot{z} &= z + \sin{t} - \cos{t}} \) % \( x = C_1e^{t} + t^2 e^t, ~ y = C_2 e^{t} + C_3 t e^{t} - 1, ~ z = C_3 e^{t} + \sin{t} \)
			\itemdstar \( \syst{\dot{x} &= \frac{1}{t^2} - \frac{1}{t} - x, \\ \dot{y} &= 2t - \ln{t} - z, \\ \dot{z} &= y - t^2 - \frac{1}{t}} \) % \( x = C_1e^{-t} + \frac{1}{t}, ~ y = C_2 \cos{t} - C_3 \sin{t} - t^2, ~ z = C_2 \sin{t} + C_3 \cos{t} + \ln{t} \)
			\itemdstar \( \syst{\dot{x} &= 4x + 2y + 2z - \frac{2}{t} + 2\tan{t}, \\ \dot{y} &= \frac{3}{t} - \frac{1}{t^2} - 5x - 3y - 2z - 2 \tan{t}, \\ \dot{z} &= y - \frac{1}{t} - \sec^2{t}} \) % \( x = C_2 e^{t} \pares{\sin{t} - \cos{t}} + C_3 e^{t} \pares{\sin{t} + \cos{t}}, ~ y = -C_1 e^{-t} + C_2 e^{t} \pares{\cos{t} - \sin{t}} - C_3 e^{t} \pares{\sin{t} + \cos{t}} - \frac{1}{t}, ~ z = C_1 e^{-t} + C_2 e^{t} \cos{t} - C_3 e^{t} \sin{t} + \tan{t} \)

		\end{enumtasks}
	\end{multicols}